lean4/Automaton/Language/Basic.lean
@@ -3,7 +3,7 @@ import Mathlib.Init.Set
 variable (Sigma : Type _)
 
 @[reducible]
-def word : Type := List Sigma
+def word : Type _ := List Sigma
 
 @[reducible]
-def Lang : Type := Set (word Sigma)
+def Lang : Type _ := Set (word Sigma)
