lean4/Automaton/DFA/ToNFA.lean
@@ -13,7 +13,7 @@ open DFA NFA
 
 namespace ToNFA
 
-variable {α : Type _} {σ : Type _} [DecidableEq α] (td sd : DFA σ) (tn sn : NFA σ)
+variable {σ : Type _} [FinEnum σ] (td sd : DFA σ) (tn sn : NFA σ)
 
 -- dfa and nfa accept the same language
 def dfa_nfa_eq : Prop := ∀ w : word σ , nfa_accepts tn w ↔ dfa_accepts td w
@@ -32,12 +32,19 @@ theorem dfa_to_nfa_eq_init : td.init = (dfa_to_nfa td).init := by dsimp [dfa_to_
 theorem dfa_to_nfa_eq_final : td.fs = (dfa_to_nfa td).fs := by dsimp[dfa_to_nfa]
 
 -- the δ_star function remains the same (but NFA produces singletons)
-theorem dfa_to_nfa_eq_δ_star  (w : word σ) : {DFA.δ_star td w} = NFA.δ_star (dfa_to_nfa td) w := by
+theorem dfa_to_nfa_eq_δ_star' (w : word σ) : (q : td.q) → {DFA.δ_star' td q w} = NFA.δ_star' (dfa_to_nfa td) {q} w := by
   induction w with
-  | nil => dsimp [DFA.δ_star,NFA.δ_star]; rw [←dfa_to_nfa_eq_init]
-  | cons a as h => dsimp [DFA.δ_star,NFA.δ_star] 
-                   rw [←h];
-                   simp [δ_step,dfa_to_nfa,dfa_δ_to_nfa_δ]              
+  | nil => intro q; simp [DFA.δ_star,NFA.δ_star]
+  | cons a as h => intro q
+                   simp [DFA.δ_star,NFA.δ_star]
+                   rw [h];
+                   simp [δ_step,dfa_to_nfa,dfa_δ_to_nfa_δ]     
+
+theorem dfa_to_nfa_eq_δ_star (w : word σ) : {DFA.δ_star td w} = NFA.δ_star (dfa_to_nfa td) w := by
+  simp [DFA.δ_star, NFA.δ_star]
+  have h : (dfa_to_nfa td).init = td.init := by simp [dfa_to_nfa]
+  rw [h]
+  apply dfa_to_nfa_eq_δ_star'
 
 -- converted dfa accepts the same language as the original dfa
 theorem dfa_to_nfa_eq : dfa_nfa_eq td (dfa_to_nfa td) := by
@@ -47,13 +54,13 @@ theorem dfa_to_nfa_eq : dfa_nfa_eq td (dfa_to_nfa td) := by
   · intro h
     simp [nfa_accepts] at h
     simp [dfa_accepts]
-    rw [←(dfa_to_nfa_eq_δ_star td w)] at h
+    rw [←(dfa_to_nfa_eq_δ_star' td w)] at h
     apply Finset.nonempty_inter_singleton_imp_in
     exact h
   · intro h
     simp [nfa_accepts]
     simp [dfa_accepts] at h
-    rw [←(dfa_to_nfa_eq_δ_star td w)]
+    rw [←(dfa_to_nfa_eq_δ_star' td w)]
     simp [dfa_to_nfa]
     rw [Finset.singleton_inter_of_mem h]
     exact (Finset.singleton_nonempty (DFA.δ_star td w))
