lean4/Automaton/NFA/Examples.lean
@@ -1,0 +1,52 @@
+import Automaton.NFA.Basic
+import Automaton.DFA.ToNFA
+import Automaton.NFA.ToDFA
+
+-- normal automaton
+
+open NFA DFA
+
+def δ₁ : Fin 2 → Fin 2 → Finset (Fin 2)
+  | 0 , 1 => {1}
+  | 0 , 0 => {0}
+  | 1 , 1 => {1}
+  | 1 , 0 => {0}
+
+def nfa₁ : NFA (Fin 2) := {q := Fin 2, init := 0 , fs := {1} , δ := δ₁}
+
+def w₁ : word (Fin 2) := []
+def w₂ : word (Fin 2) := [1 , 0]
+def w₃ : word (Fin 2) := [0 , 1]
+
+#eval nfa_accepts nfa₁ w₁
+#eval nfa_accepts nfa₁ w₂
+#eval nfa_accepts nfa₁ w₃
+
+#eval dfa_accepts (ToDFA.nfa_to_dfa nfa₁) w₁
+#eval dfa_accepts (ToDFA.nfa_to_dfa nfa₁) w₂
+#eval dfa_accepts (ToDFA.nfa_to_dfa nfa₁) w₃
+
+#eval nfa_accepts (ToNFA.dfa_to_nfa (ToDFA.nfa_to_dfa nfa₁)) w₁
+#eval nfa_accepts (ToNFA.dfa_to_nfa (ToDFA.nfa_to_dfa nfa₁)) w₂
+#eval nfa_accepts (ToNFA.dfa_to_nfa (ToDFA.nfa_to_dfa nfa₁)) w₃
+
+
+-- all strings ending with 01
+def δ₂ : Fin 4 → Fin 2 → Finset (Fin 4)
+  | 0 , 0 => {0 , 1}
+  | 0 , 1 => {0}
+  | 1 , 0 => {3}
+  | 1 , 1 => {2}
+  | _ , _ => {3}
+
+def nfa₂ : NFA (Fin 2) := {q := Fin 4, init := 0 , fs := {2} , δ := δ₂}
+
+def w₄ : word (Fin 2) := [0 , 1]
+def w₅ : word (Fin 2) := [1 , 0 , 0 , 1]
+def w₆ : word (Fin 2) := [1 , 0]
+def w₇ : word (Fin 2) := [1 , 1]
+
+#eval nfa_accepts nfa₂ w₄
+#eval nfa_accepts nfa₂ w₅
+#eval nfa_accepts nfa₂ w₆
+#eval nfa_accepts nfa₂ w₇
